added ordering at the type level, i.e. iso and galois. TimeStateMonad is proper in that it respects galois connections (the way HoTT function morphisms respect iso)

src/AAI/Classes/Transition.v
@@ -1,5 +1,14 @@
 Require Import FP.Classes.Monad.
+Require Import FP.Classes.Galois.
+Require Import FP.Classes.ProperFunctor.
 Require Import FP.Core.
 
-Class Transition (ss:qtype -> qtype) m `{! Monad m } :=
-  { transition : forall {A B}, dom ((A ⇒ m B) ⇒ (ss A ⇒ ss B)) }.
+Class Transition m `{! Monad m } :=
+  { ss : qtype -> qtype
+  ; transition : forall {A B}, dom ((A ⇒ m B) ⇒ (ss A ⇒ ss B)) 
+  }.
+Arguments ss m {Monad0 Transition} _.
+Global Opaque ss.
+
+Class GaloisTransition m₁ m₂ `{! Monad m₁ ,! Transition m₁ ,! Monad m₂ ,! Transition m₂ } :=
+  { GaloisTransition_GaloisFunctor :> GaloisFunctor (ss m₁) (ss m₂) }.
