src/AAI/Data/TimeStateMonad.v
@@ -1,41 +1,144 @@
 Require Import FP.Core.
 Require Import FP.Data.Product.
+Require Import FP.Data.Unit.
+Require Import FP.Data.StateMonad.
 Require Import FP.Classes.Monad.
+Require Import FP.Classes.Injection.
+Require Import FP.Classes.ProperFunctor.
+Require Import FP.Classes.Galois.
 Require Import AAI.Classes.MonadTimeState.
+Require Import AAI.Classes.Transition.
 
-Inductive v_timeStateMonadT (t:qtype) (m:qtype -> qtype) (a:qtype) :=
+Inductive v_timeStateMonadT (T:qtype) (m:qtype -> qtype) (A:qtype) :=
   v_TimeStateMonadT
-  { v_unTimeStateMonadT : dom (t ⇒ m (a × t)) }.
-Arguments v_TimeStateMonadT {t m a} _.
-Arguments v_unTimeStateMonadT {t m a} _.
+  { v_unTimeStateMonadT : dom (stateMonadT T m A) }.
+Arguments v_TimeStateMonadT {T m A} _.
+Arguments v_unTimeStateMonadT {T m A} _.
 
-Instance : forall t m a, Eqv (v_timeStateMonadT t m a) :=
-  { eqv x y := eqv (v_unTimeStateMonadT x) (v_unTimeStateMonadT y) }.
-Proof.
-  constructor ; simpl ; intros.
-  - LibReflexivity.
-  - Symmetry ; auto.
-  - Transitivity (v_unTimeStateMonadT y) ; auto.
-Defined.
+Definition timeStateMonadT T m A := derive (v_timeStateMonadT T m A) v_unTimeStateMonadT.
 
-Instance : forall t m a, Lte (v_timeStateMonadT t m a) :=
-  { lte x y := lte (v_unTimeStateMonadT x) (v_unTimeStateMonadT y) }.
-Proof.
-  constructor ; simpl ; intros.
-  - Reflexivity ; auto.
-  - Transitivity (v_unTimeStateMonadT y) ; auto.
-Defined.
+Definition TimeStateMonadT {T m A} : dom (stateMonadT T m A ⇒ timeStateMonadT T m A) := 
+  λ aM → v_TimeStateMonadT aM : dom (timeStateMonadT T m A).
+Definition unTimeStateMonadT {T m A} : dom (timeStateMonadT T m A ⇒ stateMonadT T m A) :=
+  λ aM → (v_unTimeStateMonadT : dom (timeStateMonadT T m A) -> _) aM.
+Instance : forall T m A, InjectionEqv (@unTimeStateMonadT T m A) :=
+  { injectionEqv _x _y p := p }.
+Instance : forall T m A, InjectionLte (@unTimeStateMonadT T m A) :=
+  { injectionLte _x _y p := p }.
+Global Opaque TimeStateMonadT.
+Global Opaque unTimeStateMonadT.
+Definition TimeStateMonadT_inv {T m A} (aM:dom (stateMonadT T m A))
+: unTimeStateMonadT ∙ (TimeStateMonadT ∙ aM) ≃ aM := libReflexivity.
+Ltac TimeStateMonadRewrite :=
+  match goal with
+  |- ⟨ unTimeStateMonadT ∙ (TimeStateMonadT ∙ ?aM) ∈ _ |_| _ ⟩ => ReplaceBy (TimeStateMonadT_inv aM)
+  end.
+  
+Section TimeStateMonadT.
+  Context {T:qtype} {m} `{! Monad m }.
 
-Definition timeStateMonadT t m a : qtype :=
-  {| qdom := v_timeStateMonadT t m a |}.
+  Definition runTimeStateMonadT {A} : dom (T ⇒ timeStateMonadT T m A ⇒ m (A × T)) :=
+    λ t → runStateMonadT ∙ t ⊙ unTimeStateMonadT.
+  
+  Definition timeStateMonadT_ret {A} : dom (A ⇒ timeStateMonadT T m A) :=
+    λ a → TimeStateMonadT $ (ret ∙ a : dom (stateMonadT T m A)).
+  Definition timeStateMonadT_bind {A B} 
+  : dom (timeStateMonadT T m A ⇒ (A ⇒ timeStateMonadT T m B) ⇒ timeStateMonadT T m B) :=
+    λ aM f → TimeStateMonadT ∙ ( 
+      a ← unTimeStateMonadT ∙ aM ;;
+      unTimeStateMonadT $ f ∙ a).
+  Global Instance : Monad (timeStateMonadT T m) :=
+    { ret := @timeStateMonadT_ret
+    ; bind := @timeStateMonadT_bind
+    }.
+  Proof.
+    Local Ltac Hammer :=
+      repeat 
+        (Re fail || MonadRewrite || TimeStateMonadRewrite ; qproper_elim).
+    - simpl ; intros.
+      apply (injectionEqv unTimeStateMonadT) ; Hammer.
+      Transitivity (bind ∙ (unTimeStateMonadT ∙ aM) ∙ ret) ; qproper_elim ; Hammer.
+    - simpl ; intros.
+      apply (injectionEqv unTimeStateMonadT) ; Hammer.
+    - simpl ; intros ; Hammer.
+  Defined.
+  
+  Definition timeStateMonadT_getTime : dom (timeStateMonadT T m T) :=
+    TimeStateMonadT $ get.
+  Definition timeStateMonadT_putTime : dom (T ⇒ timeStateMonadT T m unit) :=
+    λ t → TimeStateMonadT $ put ∙ t.
+  Global Instance : MonadTimeState T (timeStateMonadT T m) :=
+    { getTime := @timeStateMonadT_getTime
+    ; putTime := @timeStateMonadT_putTime
+    }.
+  
+  Context `{! Transition m }.
 
-Definition TimeStateMonadT {t m a} : dom ((t ⇒ m (a × t)) ⇒ timeStateMonadT t m a) := qλ f → (v_TimeStateMonadT f : dom (timeStateMonadT t m a)).
+  Definition timeStateMonadT_ss A := ss m (A × T).
+  Definition timeStateMonadT_transition {A B} 
+  : dom ((A ⇒ timeStateMonadT T m B) ⇒ (timeStateMonadT_ss A ⇒ timeStateMonadT_ss B)) :=
+    λ f → transition $ λ axt → 
+     prod_elim ∙ axt $ λ a t → 
+       runTimeStateMonadT ∙ t ∙ (f ∙ a).
 
-Definition timeStateMonadT_ret {t m a} `{! Monad m } 
-: dom (a ⇒ timeStateMonadT t m a) :=
-  qλ a → TimeStateMonadT ∙ (qλ t → ret ∙ (a ,, t)).
+  Global Instance : Transition (timeStateMonadT T m) :=
+    { ss := timeStateMonadT_ss
+    ; transition := @timeStateMonadT_transition 
+    }.
+  
+End TimeStateMonadT.
 
-Instance : forall t m, Monad (timeStateMonadT t m) :=
-  { 
+Section Galois.
+  Context {T₁ m₁ T₂ m₂} 
+  `{! Monad m₁ ,! Transition m₁ ,! Monad m₂ ,! Transition m₂ ,! Galois T₁ T₂ }.
 
-Instance : forall t m, MonadTimeState t (TimeStateMonadT t m).
+  Section GaloisFunctor.
+    Context `{! GaloisFunctor m₁ m₂ }.
+
+    Definition timeStateMonadT_galoisα {A₁ A₂} `{! Galois A₁ A₂ } 
+    : dom (timeStateMonadT T₁ m₁ A₁ ⇒ timeStateMonadT T₂ m₂ A₂) :=
+      λ aM₁ → TimeStateMonadT $ StateMonadT $ λ t₂ →
+          galoisα ∙ (runTimeStateMonadT ∙ (galoisγ ∙ t₂) ∙ aM₁).
+    Definition timeStateMonadT_galoisγ {A₁ A₂} `{! Galois A₁ A₂ }
+    : dom (timeStateMonadT T₂ m₂ A₂ ⇒ timeStateMonadT T₁ m₁ A₁) :=
+      λ aM₂ → TimeStateMonadT $ StateMonadT $ λ t₁ →
+          galoisγ ∙ (runTimeStateMonadT ∙ (galoisα ∙ t₁) ∙ aM₂).
+    Local Instance 
+    : forall A₁ A₂, Galois A₁ A₂ -> Galois (timeStateMonadT T₁ m₁ A₁) (timeStateMonadT T₂ m₂ A₂) :=
+      { galoisα := timeStateMonadT_galoisα
+      ; galoisγ := timeStateMonadT_galoisγ
+      }.
+    Proof.
+      Local Ltac Hammer := repeat 
+        (Re fail || GaloisRewrite || StateMonadRewrite || TimeStateMonadRewrite ; qproper_elim).
+      - Hammer.
+        apply (injectionLte unTimeStateMonadT) ; Hammer.
+        apply (injectionLte unStateMonadT) ; Hammer.
+      - Hammer.
+        apply (injectionLte unTimeStateMonadT) ; Hammer.
+        apply (injectionLte unStateMonadT) ; Hammer.
+    Defined.
+    Global Instance : GaloisFunctor (timeStateMonadT T₁ m₁) (timeStateMonadT T₂ m₂) := {}.
+  End GaloisFunctor.
+  
+  Section GaloisTransition.
+    Context `{! GaloisTransition m₁ m₂ }.
+
+    Local Instance
+    : forall A₁ A₂, Galois A₁ A₂ -> 
+      Galois (ss (timeStateMonadT T₁ m₁) A₁) (ss (timeStateMonadT T₂ m₂) A₂) :=
+        { galoisα := galoisα (A:=ss m₁ (A₁ × T₁)) (B:=ss m₂ (A₂ × T₂))
+        ; galoisγ := galoisγ : dom (ss m₂ (A₂ × T₂) ⇒ ss m₁ (A₁ × T₁))
+        }.
+    Proof.
+      Local Ltac Hammer := repeat
+        (Re fail || GaloisRewrite ; qproper_elim).
+      - Hammer.
+        apply qmonotonic_intro ; Hammer.
+      - Hammer.
+        apply qmonotonic_intro ; Hammer.
+    Defined.
+    Local Instance : GaloisFunctor (ss (timeStateMonadT T₁ m₁)) (ss (timeStateMonadT T₂ m₂)) := {}.
+    Global Instance : GaloisTransition (timeStateMonadT T₁ m₁) (timeStateMonadT T₂ m₂) := {}.
+  End GaloisTransition.
+End Galois.
