src/FP/Classes/Galois.v
@@ -1,25 +1,39 @@
 Require Import FP.Core.
 
 Class Galois (A B:qtype) :=
-  { galoisβ : dom (A ⇒ B)
-  ; galoisα : dom (B ⇒ A)
-  ; galois_idL : (galoisβ ⊙ galoisα) ⊑ id
-  ; galois_idR : id ⊑ (galoisα ⊙ galoisβ)
+  { galoisα : dom (A ⇒ B)
+  ; galoisγ : dom (B ⇒ A)
+  ; galois_id_αγ : (galoisα ⊙ galoisγ) ⊑ id
+  ; galois_id_γα : id ⊑ (galoisγ ⊙ galoisα)
   }.
+Global Opaque galoisα.
+Global Opaque galoisγ.
+
+Ltac GaloisRewrite :=
+  match goal with
+  | |- ⟨ (galoisα (A:=?A) (B:=?B)) ⊙ (galoisγ (A:=?A) (B:=?B)) ∈ _ |LTE| _ ⟩ =>
+      WeakenBy (galois_id_αγ (A:=A) (B:=B))
+  | |- ⟨ galoisα ∙ (galoisγ ∙ ?e) ∈ _ |LTE| _ ⟩ => 
+      WeakenBy (qmonotonic_elim galois_id_αγ e e libReflexivity)
+  | |- ⟨ (galoisγ (A:=?A) (B:=?B)) ⊙ (galoisα (A:=?A) (B:=?B)) ∈ _ |GTE| _ ⟩ =>
+      StrengthenBy (galois_id_γα (A:=A) (B:=B))
+  | |- ⟨ galoisγ ∙ (galoisα ∙ ?e) ∈ _ |GTE| _ ⟩ =>
+      StrengthenBy (qmonotonic_elim galois_id_γα e e libReflexivity)
+  end.
 
 Instance : forall A B `{! Galois A B }, Galois (A ⇒ A) (B ⇒ B) :=
-  { galoisβ := λ f → galoisβ ⊙ f ⊙ galoisα
-  ; galoisα := λ g → galoisα ⊙ g ⊙ galoisβ
+  { galoisα := λ f → galoisα ⊙ f ⊙ galoisγ
+  ; galoisγ := λ g → galoisγ ⊙ g ⊙ galoisα
   }.
 Proof.
   - qproper.
-    Transitivity (x ∙ (galoisβ ∙ (galoisα ∙ x0))).
-    + eapply (qmonotonic_elim galois_idL) ; LibReflexivity.
+    Transitivity (x ∙ (galoisα ∙ (galoisγ ∙ x0))).
+    + eapply (qmonotonic_elim galois_id_αγ) ; LibReflexivity.
     + qproper_elim.
-      eapply (qmonotonic_elim galois_idL) ; auto.
+      eapply (qmonotonic_elim galois_id_αγ) ; auto.
   - qproper.
-    Transitivity (y ∙ (galoisα ∙ (galoisβ ∙ y0))).
+    Transitivity (y ∙ (galoisγ ∙ (galoisα ∙ y0))).
     + qproper_elim.
-      eapply (qmonotonic_elim galois_idR) ; auto.
-    + eapply (qmonotonic_elim galois_idR) ; LibReflexivity.
+      eapply (qmonotonic_elim galois_id_γα) ; auto.
+    + eapply (qmonotonic_elim galois_id_γα) ; LibReflexivity.
 Defined.
