src/FP/Classes/Injection.v
@@ -1,7 +1,15 @@
 Require Import FP.Core.
 
-Class Injection {A B} (inj:dom (A ⇒ B)) :=
-  { injection : forall {x y}, inj ∙ x ≃ inj ∙ y -> x ≃ y }.
-Arguments injection {A B} inj {Injection x y} _.
+Class InjectionEqv {A B} (inj:dom (A ⇒ B)) :=
+  { injectionEqv : forall {x y}, inj ∙ x ≃ inj ∙ y -> x ≃ y }.
+Arguments injectionEqv {A B} inj {InjectionEqv x y} _.
 
-Ltac Injection f := apply (injection f).
+Class InjectionLte {A B} (inj:dom (A ⇒ B)) :=
+  { injectionLte : forall {x y}, inj ∙ x ⊑ inj ∙ y -> x ⊑ y }.
+Arguments injectionLte {A B} inj {InjectionLte x y} _.
+
+Ltac Injection f := 
+  match goal with
+  | |- _ ≃ _ => apply (injectionEqv f)
+  | |- _ ⊑ _ => apply (injectionLte f)
+  end.
