src/FP/Data/StateMonad.v
@@ -1,5 +1,6 @@
 Require Import FP.Core.
 Require Import FP.Data.Product.
+Require Import FP.Data.Unit.
 Require Import FP.Classes.Monad.
 Require Import FP.Classes.Injection.
 
@@ -10,49 +11,64 @@ Arguments v_StateMonadT {S m A} _.
 Arguments v_unStateMonadT {S m A} _.
 
 Definition stateMonadT S m A := derive (v_stateMonadT S m A) v_unStateMonadT.
+
 Definition StateMonadT {S m A} : dom ((S ⇒ m (A × S)) ⇒ stateMonadT S m A) :=
   λ f → (v_StateMonadT f : dom (stateMonadT S m A)).
 Definition unStateMonadT {S m A} : dom (stateMonadT S m A ⇒ S ⇒ m (A × S)) :=
   λ aM → v_unStateMonadT (aM : dom (stateMonadT S m A)).
-Arguments unStateMonadT : simpl never.
-Instance : forall S m A, Injection (@unStateMonadT S m A) :=
-  { injection _x _y p := p }.
+Instance : forall S m A, InjectionEqv (@unStateMonadT S m A) :=
+  { injectionEqv _x _y p := p }.
+Instance : forall S m A, InjectionLte (@unStateMonadT S m A) :=
+  { injectionLte _x _y p := p }.
 Global Opaque StateMonadT.
 Global Opaque unStateMonadT.
 Definition StateMonadT_inv {S m A} (f:dom (S ⇒ m (A × S))) 
-: (@unStateMonadT S m A) ∙ (StateMonadT ∙ f) ≃ f := libReflexivity f.
+: unStateMonadT ∙ (StateMonadT ∙ f) ≃ f := libReflexivity.
 Ltac StateMonadRewrite :=
   match goal with
-  |- ⟨ unStateMonadT ∙ (StateMonadT ∙ ?f) ∈ _ ⋈ _ ⟩ => ReplaceBy (StateMonadT_inv f)
+  |- ⟨ unStateMonadT ∙ (StateMonadT ∙ ?f) ∈ _ |_| _ ⟩ => ReplaceBy (StateMonadT_inv f)
   end.
-  
-Definition runStateMonadT {S m A} : dom (S ⇒ stateMonadT S m A ⇒ m (A × S)) :=
-  λ x aM → unStateMonadT ∙ aM ∙ x.
 
-Definition stateMonadT_ret {S m} `{! Monad m } {A} : dom (A ⇒ stateMonadT S m A) :=
-  λ a → StateMonadT $ λ s → ret ∙ (a ,, s).
-Definition stateMonadT_bind {S m} `{! Monad m } {A B}
-: dom (stateMonadT S m A ⇒ (A ⇒ stateMonadT S m B) ⇒ stateMonadT S m B) :=
-  λ aM k → StateMonadT $ λ s →
-    axs ← runStateMonadT ∙ s ∙ aM ;;
-    prod_elim ∙ axs $ λ a s →
-    runStateMonadT ∙ s ∙ (k ∙ a).
-    
-Instance : forall S m `{! Monad m }, Monad (stateMonadT S m) :=
-  { ret := @stateMonadT_ret S m _
-  ; bind := @stateMonadT_bind S m _
-  }.
-Proof.
-  Local Ltac Hammer := 
-    repeat
-      (Re fail || ProdRewrite || MonadRewrite || StateMonadRewrite ; qproper_elim).
-  - intros ; simpl.
-    apply (injection unStateMonadT).
-    Hammer.
-    Transitivity (bind ∙ (unStateMonadT ∙ aM ∙ y) ∙ ret) ; qproper_elim ; Hammer.
-  - intros ; simpl.
-    apply (injection unStateMonadT).
-    Hammer.
-  - intros ; simpl.
-    Hammer.
-Defined.
+Section StateMonadT.
+  Context {S:qtype} {m:qtype -> qtype} `{! Monad m }.
+
+  Definition runStateMonadT {A} : dom (S ⇒ stateMonadT S m A ⇒ m (A × S)) :=
+    λ x aM → unStateMonadT ∙ aM ∙ x.
+
+  Definition stateMonadT_ret {A} : dom (A ⇒ stateMonadT S m A) :=
+    λ a → StateMonadT $ λ s → ret ∙ (a ,, s).
+  Definition stateMonadT_bind {A B}
+  : dom (stateMonadT S m A ⇒ (A ⇒ stateMonadT S m B) ⇒ stateMonadT S m B) :=
+    λ aM k → StateMonadT $ λ s →
+      axs ← runStateMonadT ∙ s ∙ aM ;;
+      prod_elim ∙ axs $ λ a s →
+      runStateMonadT ∙ s ∙ (k ∙ a).
+
+  Global Instance : Monad (stateMonadT S m) :=
+    { ret := @stateMonadT_ret
+    ; bind := @stateMonadT_bind
+    }.
+  Proof.
+    Local Ltac Hammer := 
+      repeat
+        (Re fail || ProdRewrite || MonadRewrite || StateMonadRewrite ; qproper_elim).
+    - intros ; simpl.
+      apply (injectionEqv unStateMonadT).
+      Hammer.
+      Transitivity (bind ∙ (unStateMonadT ∙ aM ∙ y) ∙ ret) ; qproper_elim ; Hammer.
+    - intros ; simpl.
+      apply (injectionEqv unStateMonadT).
+      Hammer.
+    - intros ; simpl.
+      Hammer.
+  Defined.
+
+  Definition stateMonadT_get : dom (stateMonadT S m S) :=
+    StateMonadT $ λ s → ret ∙ (s ,, s).
+  Definition stateMonadT_put : dom (S ⇒ stateMonadT S m unit) :=
+    λ s → StateMonadT $ λ _ → ret ∙ (tt ,, s).
+  Global Instance : MonadState S (stateMonadT S m) :=
+    { get := stateMonadT_get
+    ; put := stateMonadT_put
+    }.
+End StateMonadT.
