src/AAI/Classes/MonadTimeState.v
@@ -2,16 +2,15 @@ Require Import FP.Core.
 Require Import FP.Classes.Monad.
 Require Import FP.Data.Unit.
 
-
 Class MonadTimeState T m :=
   { getTime : dom (m T)
-  ; putTime : dom (T ⇒ m qunit)
+  ; putTime : dom (T ⇒ m unit)
   }.
 
 Section MonadTimeState.
   Context {T m} `{! Monad m ,! MonadTimeState T m }.
 
-  Definition modifyTime : dom ((T ⇒ T) ⇒ m qunit) := λ f →
+  Definition modifyTime : dom ((T ⇒ T) ⇒ m unit) := λ f →
     e ← getTime ;;
     putTime $ f ∙ e.
 End MonadTimeState.
