src/FP/Classes/Iso.v
@@ -1,0 +1,8 @@
+Require Import FP.Core.
+
+Class Iso A B :=
+  { isoTo : dom (A ⇒ B)
+  ; isoFrom : dom (B ⇒ A)
+  ; iso_to_from : (isoTo ⊙ isoFrom) ≃ id
+  ; iso_from_to : (isoFrom ⊙ isoTo) ≃ id
+  }.
