src/FP/Classes/ProperFunctor.v
@@ -1,0 +1,12 @@
+Require Import FP.Core.
+Require Import FP.Classes.Iso.
+Require Import FP.Classes.Galois.
+
+Class IsoFunctor (t:qtype -> qtype) (u:qtype -> qtype) :=
+  { IsoFunctor_Iso :> forall {A B}, Iso A B -> Iso (t A) (u B) }.
+Class GaloisFunctor (t:qtype -> qtype) (u:qtype -> qtype) :=
+  { GaloisFunctor_Galois :> forall {A B}, Galois A B -> Galois (t A) (u B) }.
+Class ProperFunctor (t:qtype -> qtype) :=
+  { ProperFunctor_Iso :> IsoFunctor t t
+  ; ProperFunctor_Galois :> GaloisFunctor t t
+  }.
