src/FP/Core/Rewrite.v
@@ -9,63 +9,118 @@ Definition focusFun {A B C} (x:dom A) (k:dom (B ⇒ C)) : dom ((A ⇒ B) ⇒ C) 
 Definition focusArg {A B C} (f:dom (A ⇒ B)) (k:dom (B ⇒ C)) : dom (A ⇒ C) :=
   k ⊙ apply ∙ f.
 
-Definition state {A B:qtype} (x:dom A) (k:dom (A ⇒ B)) (y:dom B) := 
-  k ∙ x ≃ y.
+Inductive mode := EQV | LTE | GTE.
+
+Definition state {A B:qtype} (m:mode) :=
+  match m with
+  | EQV => fun (x:dom A) (k:dom (A ⇒ B)) (y:dom B) => k ∙ x ≃ y
+  | LTE => fun (x:dom A) (k:dom (A ⇒ B)) (y:dom B) => k ∙ x ⊑ y
+  | GTE => fun (x:dom A) (k:dom (A ⇒ B)) (y:dom B) => y ⊑ k ∙ x
+  end.
+
 Opaque state.
 
 Notation "⊤κ" := topk.
 Infix "◁" := focusFun (at level 60, right associativity).
 Infix "▷" := focusArg (at level 60, right associativity).
-Notation "⟨ x ∈ k ⋈ y ⟩" := (state x k y).
+Notation "⟨ x ∈ k | m | y ⟩" := (state m x k y).
 
-Ltac Enter :=
+Ltac EnterLeft :=
   match goal with
-  |- ?x ≃ ?y => change ⟨ x ∈ ⊤κ ⋈ y ⟩
+  | |- ?x ≃ ?y => change ⟨ x ∈ ⊤κ |EQV| y ⟩
+  | |- ?x ⊑ ?y => change ⟨ x ∈ ⊤κ |LTE| y ⟩
   end.
-Ltac Exit :=
+Ltac ExitLeft :=
   match goal with
-  |- ⟨ ?x ∈ ⊤κ ⋈ ?y ⟩ => change (x ≃ y)
+  | |- ⟨ ?x ∈ ⊤κ |EQV| ?y ⟩ => change (x ≃ y)
+  | |- ⟨ ?x ∈ ⊤κ |LTE| ?y ⟩ => change (x ⊑ y)
   end.
+Ltac EnterRight :=
+  match goal with
+  | |- ?x ≃ ?y => Symmetry ; change ⟨ y ∈ ⊤κ |EQV| x ⟩
+  | |- ?x ⊑ ?y => change ⟨ y ∈ ⊤κ |GTE| x ⟩
+  end.
+Ltac ExitRight :=
+  match goal with
+  | |- ⟨ ?y ∈ ⊤κ |EQV| ?x ⟩ => change (y ≃ x) ; Symmetry
+  | |- ⟨ ?y ∈ ⊤κ |GTE| ?x ⟩ => change (x ⊑ y)
+  end.
+
 Ltac PushFun :=
   match goal with
-  |- ⟨ ?f ∙ ?x ∈ ?k ⋈ ?y ⟩ => change ⟨ f ∈ (x ◁ k) ⋈ y ⟩
+  | |- ⟨ ?f ∙ ?x ∈ ?k |EQV| ?y ⟩ => change ⟨ f ∈ (x ◁ k) |EQV| y ⟩
+  | |- ⟨ ?f ∙ ?x ∈ ?k |LTE| ?y ⟩ => change ⟨ f ∈ (x ◁ k) |LTE| y ⟩
+  | |- ⟨ ?f ∙ ?x ∈ ?k |GTE| ?y ⟩ => change ⟨ f ∈ (x ◁ k) |GTE| y ⟩
   end.
 Ltac PopFun :=
   match goal with
-  |- ⟨ ?f ∈ (?x ◁ ?k) ⋈ ?y ⟩ => change ⟨ f ∙ x ∈ k ⋈ y ⟩
+  | |- ⟨ ?f ∈ (?x ◁ ?k) |EQV| ?y ⟩ => change ⟨ f ∙ x ∈ k |EQV| y ⟩
+  | |- ⟨ ?f ∈ (?x ◁ ?k) |LTE| ?y ⟩ => change ⟨ f ∙ x ∈ k |LTE| y ⟩
+  | |- ⟨ ?f ∈ (?x ◁ ?k) |GTE| ?y ⟩ => change ⟨ f ∙ x ∈ k |GTE| y ⟩
   end.
 Ltac PushArg :=
   match goal with
-  |- ⟨ ?f ∙ ?x ∈ ?k ⋈ ?y ⟩ => change ⟨ x ∈ (f ▷ k) ⋈ y ⟩
+  | |- ⟨ ?f ∙ ?x ∈ ?k |EQV| ?y ⟩ => change ⟨ x ∈ (f ▷ k) |EQV| y ⟩
+  | |- ⟨ ?f ∙ ?x ∈ ?k |LTE| ?y ⟩ => change ⟨ x ∈ (f ▷ k) |LTE| y ⟩
+  | |- ⟨ ?f ∙ ?x ∈ ?k |GTE| ?y ⟩ => change ⟨ x ∈ (f ▷ k) |GTE| y ⟩
   end.
 Ltac PopArg :=
   match goal with
-  |-  ⟨ ?x ∈ (?f ▷ ?k) ⋈ ?y ⟩ => change ⟨ f ∙ x ∈ k ⋈ y ⟩
+  | |-  ⟨ ?x ∈ (?f ▷ ?k) |EQV| ?y ⟩ => change ⟨ f ∙ x ∈ k |EQV| y ⟩
+  | |-  ⟨ ?x ∈ (?f ▷ ?k) |LTE| ?y ⟩ => change ⟨ f ∙ x ∈ k |LTE| y ⟩
+  | |-  ⟨ ?x ∈ (?f ▷ ?k) |GTE| ?y ⟩ => change ⟨ f ∙ x ∈ k |GTE| y ⟩
   end.
 
-Definition replace {A B} {x x':dom A} {k:dom (A ⇒ B)} {y:dom B} 
-(e:x ≃ x') (g:⟨ x' ∈ k ⋈ y ⟩) : ⟨ x ∈ k ⋈ y ⟩.
+Definition eqv_replace {A B} {x x':dom A} {k:dom (A ⇒ B)} {y:dom B} 
+(e:x ≃ x') (g:⟨ x' ∈ k |EQV| y ⟩) : ⟨ x ∈ k |EQV| y ⟩.
 Proof.
   change (k ∙ x ≃ y).
-  Transitivity (k ∙ x').
-  - qproper_elim.
-  - exact g.
+  Transitivity (k ∙ x') ; qproper_elim.
+  exact g.
 Qed.
+Definition lte_replace_lte {A B} {x x':dom A} {k:dom (A ⇒ B)} {y:dom B}
+(e:x ⊑ x') (g:⟨ x' ∈ k |LTE| y ⟩) : ⟨ x ∈ k |LTE| y ⟩.
+Proof.
+  change (k ∙ x ⊑ y).
+  Transitivity (k ∙ x') ; qproper_elim.
+  exact g.
+Qed.
+Definition lte_replace_eqv {A B} {x x':dom A} {k:dom (A ⇒ B)} {y:dom B}
+(e:x ≃ x') : ⟨ x' ∈ k |LTE| y ⟩ -> ⟨ x ∈ k |LTE| y ⟩ := lte_replace_lte (reflexivity e).
+Definition gte_replace_gte {A B} {x x':dom A} {k:dom (A ⇒ B)} {y:dom B}
+(d:x' ⊑ x) (g:⟨ x' ∈ k |GTE| y ⟩) : ⟨ x ∈ k |GTE| y ⟩.
+Proof.
+  change (y ⊑ k ∙ x).
+  Transitivity (k ∙ x') ; qproper_elim.
+  exact g.
+Qed.
+Definition gte_replace_eqv {A B} {x x':dom A} {k:dom (A ⇒ B)} {y:dom B}
+(e:x ≃ x') : ⟨ x' ∈ k |GTE| y ⟩ -> ⟨ x ∈ k |GTE| y ⟩ := 
+  gte_replace_gte (reflexivity (symmetry e)).
 Ltac ReplaceBy p :=
   match goal with
-  |- ⟨ ?x ∈ ?k ⋈ ?y ⟩ => apply (replace p)
+  | |- ⟨ ?x ∈ ?k |EQV| ?y ⟩ => apply (eqv_replace p)
+  | |- ⟨ ?x ∈ ?k |LTE| ?y ⟩ => apply (lte_replace_eqv p)
+  | |- ⟨ ?x ∈ ?k |GTE| ?y ⟩ => apply (gte_replace_eqv p)
+  end.
+Ltac WeakenBy p :=
+  match goal with
+  | |- ⟨ ?x ∈ ?k |LTE| ?y ⟩ => apply (lte_replace_lte p)
+  end.
+Ltac StrengthenBy p :=
+  match goal with
+  | |- ⟨ ?x ∈ ?k |GTE| ?y ⟩ => apply (gte_replace_gte p)
   end.
 
 Ltac Everywhere_k t :=
   match goal with
-  | |- ⟨ _ ∙ _ ∈ _ ⋈ _ ⟩ =>
+  | |- ⟨ _ ∙ _ ∈ _ | _ | _ ⟩ =>
       chain PushFun ; Everywhere_k t ; PopFun |+|
       chain PushArg ; Everywhere_k t ; PopArg |+|
       t ; repeat t
   | _ => t ; repeat t
   end.
-Ltac Everywhere_1 t := Enter ; Everywhere_k t ; Exit.
 Ltac Everywhere t :=
-  try Everywhere_1 t ;
-  try (Symmetry ; Everywhere_1 t ; Symmetry).
+  try (EnterLeft ; Everywhere_k t ; ExitLeft) ;
+  try (EnterRight ; Everywhere_k t ; ExitRight).
 Tactic Notation "Re" tactic2(t) := Everywhere t.
