src/FP/Data/Unit.v
@@ -1,3 +1,6 @@
 Require Import FP.Core.
 
-Definition qunit := lib unit.
+Definition vunit := Coq.Init.Datatypes.unit.
+Definition vtt := Coq.Init.Datatypes.tt.
+Definition unit := lib vunit.
+Definition tt : dom unit := vtt.
